Bedrock/Platform/Cito/BoolFacts.v
@@ -12,3 +12,7 @@ Lemma bool_irre (a b : bool) (H1 H2 : a = b) : H1 = H2.
 Proof.
   eapply UIP.
 Qed.
+
+Require Import Sumbool.
+
+Definition boolcase := sumbool_of_bool.
